src/coq/MiniCProp.v
@@ -1,0 +1,196 @@
+Require Import paco.
+Require Import Bool String Ascii List.
+Require Import Omega.
+Require Import Vellvm.MiniLLVM.
+Require Import Vellvm.Util Vellvm.Misc.
+
+Import ListNotations.
+
+Set Implicit Arguments.
+
+Fixpoint subst_value id v v' :=
+  match v' with
+    | SV (VALUE_Ident _ id') => if ident_eq_dec id id' then v else SV (VALUE_Ident _ id')
+    | SV (OP_IBinop iop t vl vr) => SV (OP_IBinop iop t (subst_value id v vl) (subst_value id v vr))
+    | SV (OP_ICmp cmp t vl vr) => SV (OP_ICmp cmp t (subst_value id v vl) (subst_value id v vr))
+    | x => x
+  end.
+
+Definition subst_tvalue id v (tv : tvalue) :=
+  let '(t, v') := tv in (t, subst_value id v' v).
+
+Definition subst_instr id v (i : instr) :=
+  match i with
+    | INSTR_Op v' => INSTR_Op (subst_value id v v')
+    | INSTR_Call fn args => INSTR_Call fn (map (subst_tvalue id v) args)
+    | INSTR_Phi t args => INSTR_Phi t (map (fun x => (fst x, subst_value id v (snd x))) args)
+    | INSTR_Load t ptr => INSTR_Load t (subst_tvalue id v ptr)
+    | INSTR_Store val ptr => INSTR_Store (subst_tvalue id v val) ptr
+    | _ => i
+  end.
+
+Definition subst_term id v (t : terminator) :=
+  match t with
+    | TERM_Ret v' => TERM_Ret (subst_tvalue id v v')
+    | TERM_Br v' br1 br2 => TERM_Br (subst_tvalue id v v') br1 br2
+    | _ => t
+  end.
+
+Fixpoint subst_instr_list l i :=
+  match l with
+    | [] => i
+    | (id, v) :: t => subst_instr_list t (subst_instr id v i)
+  end.
+
+Fixpoint subst_term_list l term :=
+  match l with
+    | [] => term
+    | (id, v) :: t => subst_term_list t (subst_term id v term)
+  end.
+
+Definition get_constants_from_block (l : block) :=
+  fold_right (fun i subs =>
+                match i with
+                  | (IId id, INSTR_Op (SV (VALUE_Integer _ i) as val)) =>
+                    (ID_Local id, val) :: subs
+                  | sub => subs
+                end) [] (blk_instrs l).
+
+Definition get_constants_from_blocks (l : list block) :=
+  fold_right (fun i subs => get_constants_from_block i ++ subs) [] l.
+
+Definition get_constants es :=
+  fold_right (fun d acc =>
+                match d with
+                  | TLE_Definition d => get_constants_from_blocks (df_instrs d) ++ acc
+                end) [] es.
+
+Definition prop_const_block_instrs subs (l : list (instr_id * instr)) :=
+  fold_right (fun i l =>
+                let '(id, v) := i in
+                match (id, subst_instr_list subs v) with
+                  | (IId id, INSTR_Op (SV (VALUE_Integer _ i) as val)) =>
+                    l
+                  | sub => sub :: l
+                end) [] l.
+
+Definition remove_const_block_instrs subs (l : list (instr_id * instr)) :=
+  fold_right (fun i l =>
+                let '(id, v) := i in
+                match (subst_instr_list subs v) with
+                  | (INSTR_Op (SV (VALUE_Integer _ i) as val)) =>
+                    l
+                  | sub => (id, v) :: l
+                end) [] l.
+                    
+Definition prop_const_block subs b :=
+  {| blk_id := blk_id b;
+     blk_instrs := prop_const_block_instrs subs (blk_instrs b);
+     blk_term_id := blk_term_id b;
+     blk_term := subst_term_list subs (blk_term b)
+  |}.
+
+Definition remove_const_block subs b :=
+  {| blk_id := blk_id b;
+     blk_instrs := remove_const_block_instrs subs (blk_instrs b);
+     blk_term_id := blk_term_id b;
+     blk_term := blk_term b
+  |}.
+
+Definition prop_const_def subs d :=
+  {| df_prototype := df_prototype d;
+     df_args := df_args d;
+     df_instrs := map (prop_const_block subs) (df_instrs d)
+  |}.
+
+Definition remove_const_def subs d :=
+  {| df_prototype := df_prototype d;
+     df_args := df_args d;
+     df_instrs := map (remove_const_block subs) (df_instrs d)
+  |}.
+
+Definition prop_const_entity subs e :=
+  match e with
+    | TLE_Definition d => TLE_Definition (prop_const_def subs d)
+  end.
+
+Definition remove_const_entity subs e :=
+  match e with
+    | TLE_Definition d => TLE_Definition (remove_const_def subs d)
+  end.
+
+Definition prop_const_entities es :=
+  let constants := get_constants es in
+  map (prop_const_entity constants) es.
+
+Definition remove_const_entities es :=
+  let constants := get_constants es in
+  map (remove_const_entity constants) es.
+
+Lemma prop_const_preserve_id :
+  forall subs b, blk_id b = blk_id (prop_const_block subs b).
+Proof.
+  intros. unfold prop_const_block.
+  destruct (prop_const_block_instrs subs (blk_instrs b)); simpl; eauto. 
+Qed.
+
+Fixpoint value_to_dvalue (x : value) : dvalue :=
+  match x with
+    | SV (VALUE_Ident _ x) => DV (VALUE_Ident _ x)
+    | SV (VALUE_Integer _ i) => DV (VALUE_Integer _ i)
+    | SV (VALUE_Bool _ b) => DV (VALUE_Bool _ b)
+    | SV (VALUE_Null _) => DV (VALUE_Null _)
+    | SV (VALUE_Undef _) => DV (VALUE_Undef _)
+    | SV (OP_IBinop b t e1 e2) => DV (OP_IBinop b t (value_to_dvalue e1) (value_to_dvalue e2))
+    | SV (OP_ICmp b t e1 e2) => DV (OP_ICmp b t (value_to_dvalue e1) (value_to_dvalue e2))
+  end.
+
+Inductive wf_dvalue : dvalue -> Prop :=
+| wf_code_pointer : forall p, wf_dvalue (DVALUE_CodePointer p)
+| wf_addr : forall a, wf_dvalue (DVALUE_Addr a)
+| wf_int : forall i, wf_dvalue (DV (VALUE_Integer dvalue i))
+| wf_bool : forall b, wf_dvalue (DV (VALUE_Bool dvalue b))
+| wf_null : wf_dvalue (DV (VALUE_Null dvalue))
+| wf_undef : wf_dvalue (DV (VALUE_Undef dvalue))
+.
+
+Lemma eval_subst_env :
+  forall x i env exp,
+    wf_dvalue (value_to_dvalue x) ->
+    eval_op env (subst_value (ID_Local i) x exp) = eval_op ((i, value_to_dvalue x) :: env) exp.
+Proof.
+  intros. induction exp using value_ind'; eauto.
+  - simpl. destruct id; simpl; eauto. unfold lookup_env; simpl. simpl.
+    compare id i; try intro; try (repeat decide equality); subst.
+    + destruct (raw_id_eq_dec i i); try solve [exfalso; apply n; eauto].
+      destruct (ident_eq_dec (ID_Local i) (ID_Local i)); try solve [exfalso; apply n; eauto]. destruct x.
+      inversion H; destruct e1; inversion H1; subst; eauto.
+    + destruct (raw_id_eq_dec id i); try solve [exfalso; eauto].
+      destruct (ident_eq_dec (ID_Local i) (ID_Local id)); try solve [exfalso; inversion e; eauto].
+      simpl; eauto.
+  - simpl. rewrite IHexp1. rewrite IHexp2. eauto.
+  - simpl. rewrite IHexp1. rewrite IHexp2. eauto.
+Qed.
+
+Definition constants_to_env (e : list (ident * value)) :=
+  map (fun x => let '(id, v) := x in
+                match id with
+                  | ID_Local i
+                  | ID_Global i => (i, value_to_dvalue v)
+                end) e.
+
+Definition stepConstants subs CFG s : D state :=
+  let '(p, e, k) := s in
+  stepD CFG (p, subs ++ e, k).
+
+CoFixpoint semConstants subs CFG s : DLim :=
+  bind (stepConstants subs CFG s) (semConstants subs CFG).
+
+Lemma prop_remove_equiv :
+  forall cs es CFG1 CFG2,
+    cs = get_constants es ->
+    TLE_to_cfg (prop_const_entities es) = Some CFG1 ->
+    TLE_to_cfg (remove_const_entities es) = Some CFG2 ->
+    d_equiv (semConstants (constants_to_env cs) CFG2 (init_state CFG2)) (sem CFG1 (init_state CFG1)).
+Proof.
+Admitted.
