src/coq/MiniCfold.v
@@ -1,0 +1,200 @@
+Require Import paco.
+Require Import Bool String Ascii List.
+Require Import Omega.
+Require Import Vellvm.MiniLLVM.
+Require Import Vellvm.Util Vellvm.Misc.
+
+Set Implicit Arguments.
+
+Fixpoint cfold_val (d : value) : value :=
+  match d with
+    | SV s =>
+      match s with
+        | VALUE_Ident _ id => SV (VALUE_Ident value id)  
+        | VALUE_Integer _ x => SV (VALUE_Integer value x)
+        | VALUE_Bool _ b => SV (VALUE_Bool value b)
+        | VALUE_Null _ => SV (VALUE_Null value)
+        | VALUE_Undef _ => SV (VALUE_Undef value)
+        | OP_IBinop ib t v1 v2 =>
+          let cv1 := cfold_val v1 in
+          let cv2 := cfold_val v2 in
+          match cv1, cv2 with
+            | SV (VALUE_Integer _ x), SV (VALUE_Integer _ y) =>
+              match ib with
+                | Add => SV (VALUE_Integer value (x + y))
+                | Sub => SV (VALUE_Integer value (x - y))
+                | Mul => SV (VALUE_Integer value (x * y))
+              end
+            | _ , _ => SV (OP_IBinop ib t cv1 cv2)
+          end
+        | OP_ICmp ic t v1 v2 =>
+          let cv1 := cfold_val v1 in
+          let cv2 := cfold_val v2 in
+          match cv1, cv2 with
+            | SV (VALUE_Integer _ x), SV (VALUE_Integer _ y) =>
+              match ic with
+                | Eq => SV (VALUE_Bool value (nat_beq x y))
+                | Ule => SV (VALUE_Bool value (leb x y)) 
+              end
+            | _, _ => SV (OP_ICmp ic t cv1 cv2)
+          end
+      end
+  end.
+
+Definition cfold_instr i :=
+  match i with
+    | INSTR_Op o => INSTR_Op (cfold_val o)
+    | INSTR_Call fn args => INSTR_Call fn (map (fun p => (fst p, cfold_val (snd p))) args)
+    | INSTR_Phi t args => INSTR_Phi t (map (fun p => (fst p, cfold_val (snd p))) args)
+    | INSTR_Alloca t => INSTR_Alloca t
+    | INSTR_Load t (a, b) => INSTR_Load t (a, cfold_val b) 
+    | INSTR_Store (a, b) ptr => INSTR_Store (a, cfold_val b) ptr
+    | INSTR_Unreachable => INSTR_Unreachable
+  end.
+
+Definition cfold_term t :=                                            
+  match t with
+    | TERM_Ret (a, b) => TERM_Ret (a, cfold_val b)
+    | TERM_Ret_void => TERM_Ret_void
+    | TERM_Br (a, b) v1 v2 => TERM_Br (a, cfold_val b) v1 v2 
+    | TERM_Br_1 b => TERM_Br_1 b
+  end.
+
+Definition cfold_cmd c :=
+  match c with
+    | Step i p => Step (cfold_instr i) p
+    | Jump t => Jump (cfold_term t)
+  end.
+
+Definition cfold_phis (ps : list (local_id * instr)) :=
+  map (fun p => (fst p, cfold_instr (snd p))) ps.
+
+Definition cfold_block_entry b :=
+  match b with
+    | Phis ls p => Phis (cfold_phis ls) p
+  end.
+
+Definition cfold cfg :=
+  {|
+    init := init cfg;
+    code := fun p => match (code cfg p) with
+                       | None => None
+                       | Some x => Some (cfold_cmd x)
+                     end;
+    funs := funs cfg;
+    blks := fun fid bid =>
+              match (blks cfg fid bid) with
+                | None => None
+                | Some x => Some (cfold_block_entry x)
+              end
+  |}.
+
+Lemma cfold_eval_op_correct :
+  forall v st, eval_op st (cfold_val v) = eval_op st v.
+Proof.
+  intros. induction v using value_ind'; eauto.
+  - simpl. rewrite <- IHv1. rewrite <- IHv2.
+    destruct (cfold_val v1); eauto.
+    destruct e; eauto.
+    destruct (cfold_val v2); eauto.
+    destruct e; eauto.
+    simpl. destruct iop; eauto.
+  - simpl. rewrite <- IHv1. rewrite <- IHv2.
+    destruct (cfold_val v1); eauto.
+    destruct e; eauto.
+    destruct (cfold_val v2); eauto.
+    destruct e; eauto.
+    simpl. destruct cmp; eauto. 
+Qed.
+
+Lemma cfold_jump_correct :
+  forall cfg p e_old e ps q k,
+    jump cfg p e_old e ps q k = jump (cfold cfg) p e_old e (cfold_phis ps) q k.
+Proof.
+  intros. generalize dependent e. induction ps; eauto. destruct a. simpl.
+  intros. destruct i; eauto.
+  - simpl. rewrite assoc_map.
+    destruct (assoc ident_eq_dec (ID_Local (bn p)) args); simpl; eauto.
+    rewrite cfold_eval_op_correct; eauto.
+    destruct (eval_op e_old v); eauto. 
+  - destruct ptr. eauto.
+  - destruct ptr. destruct val; eauto.
+Qed.
+
+Lemma cfold_stepD_correct : forall CFG s, stepD CFG s = stepD (cfold CFG) s.
+Proof.
+  intros. destruct s. destruct p. destruct CFG. simpl.
+  destruct (code p); eauto; simpl.
+  destruct c; unfold cfold_cmd.
+  - destruct i; simpl; try (destruct ptr); try (destruct val); try (destruct v); eauto.
+    + destruct (def_id_of_path p); eauto; simpl.
+      rewrite cfold_eval_op_correct; eauto.
+    + destruct fn. destruct i; eauto.
+      destruct (def_id_of_path p); eauto; simpl.
+      destruct (funs id); eauto; simpl.
+      destruct p1. destruct p1.
+      destruct (map_option raw_id_of_ident l); eauto; simpl.
+      rewrite map_map.
+      rewrite map_option_map. rewrite map_option_map.
+      simpl.
+      assert (map_option (fun x => eval_op e (snd x)) args = map_option (fun x => eval_op e (cfold_val (snd x))) args).
+      induction args; eauto. simpl. rewrite cfold_eval_op_correct.
+      rewrite IHargs; eauto.
+      rewrite <- H; eauto. 
+    + rewrite cfold_eval_op_correct; eauto.
+    + rewrite cfold_eval_op_correct; eauto.
+  - destruct t; simpl; eauto.
+    + destruct v. destruct s; rewrite cfold_eval_op_correct; eauto.
+    + destruct v. destruct br1. destruct br2.
+      rewrite cfold_eval_op_correct; eauto.
+      destruct (eval_op e v); eauto. destruct d; eauto.
+      destruct e0; eauto. destruct b; simpl.
+      destruct (raw_id_of_ident i); simpl; eauto.
+      destruct (blks (bn p) r); simpl; eauto.
+      * destruct b; simpl. rewrite cfold_jump_correct; eauto.
+      * destruct (raw_id_of_ident i0); simpl; eauto.
+        destruct (blks (bn p) r); simpl; eauto.
+        destruct b; simpl. rewrite cfold_jump_correct.  eauto.
+    + destruct br. destruct (raw_id_of_ident i); simpl; eauto.
+      destruct (blks (bn p) r); simpl; eauto.
+      destruct b; simpl; rewrite cfold_jump_correct; eauto.
+Qed.
+
+Lemma cfold_init_state: forall CFG, init_state CFG = init_state (cfold CFG).
+Proof.
+  destruct CFG; eauto.
+Qed.
+
+Lemma CFG_cfold_bind_equiv :
+  forall d CFG, d_equiv (bind d (sem CFG)) (bind d (sem (cfold CFG))).
+Proof.
+  pcofix CIH. intros. pfold.
+  rewrite id_d_eq; rewrite id_d_eq at 1.
+  destruct d; try solve [constructor; eauto].
+  - constructor. rewrite sem_unfold. rewrite sem_unfold.
+    right. rewrite <- cfold_stepD_correct. apply CIH.
+  - constructor. fold (bind d (sem CFG)).
+    fold (bind d (sem (cfold CFG))). right; eapply CIH.
+  - constructor. destruct m.
+    + simpl. constructor. intro. right.
+      fold (bind (k a) (sem CFG)). fold (bind (k a) (sem (cfold CFG))).
+      eapply CIH.
+    + simpl. constructor. intro. right.
+      fold (bind (k dv) (sem CFG)). fold (bind (k dv) (sem (cfold CFG))).
+      eapply CIH.
+    + simpl. constructor. right.
+      fold (bind k (sem CFG)). fold (bind k (sem (cfold CFG))).
+      eapply CIH.
+Qed.
+
+Lemma CFG_cfold_sem_equiv : forall st CFG, d_equiv (sem CFG st) (sem (cfold CFG) st).
+Proof.
+  intros. repeat (rewrite sem_unfold). rewrite <- cfold_stepD_correct.
+  eapply CFG_cfold_bind_equiv.
+Qed.
+
+Theorem CFG_equiv_cfold : forall CFG, CFG_equiv CFG (cfold CFG).
+Proof.
+  intros. unfold CFG_equiv. rewrite <- cfold_init_state.
+  apply CFG_cfold_sem_equiv.
+Qed.
