src/coq/MiniNopRemove.v
@@ -1,0 +1,202 @@
+Require Import paco.
+Require Import Bool String Ascii List.
+Require Import Omega.
+Require Import Vellvm.MiniLLVM_nop.
+Require Import Vellvm.Util Vellvm.Misc.
+
+Import ListNotations.
+
+Set Implicit Arguments.
+
+Definition remove_nops_block_instrs (b : list (instr_id * instr)) :=
+  filter (fun x => match snd x with
+                     | INSTR_Nop => true
+                     | _ => false
+                   end) b.
+
+Definition remove_nops_block b :=
+  {| blk_id := blk_id b;
+     blk_instrs := remove_nops_block_instrs (blk_instrs b);
+     blk_term_id := blk_term_id b;
+     blk_term := blk_term b
+  |}.
+
+Definition remove_nops_def d :=
+  {| df_prototype := df_prototype d;
+     df_args := df_args d;
+     df_instrs := map remove_nops_block (df_instrs d)
+  |}.
+
+Definition remove_nops_entity e :=
+  match e with
+    | TLE_Definition d => TLE_Definition (remove_nops_def d)
+  end.
+
+Definition remove_nops_entities es :=
+  map remove_nops_entity es.
+
+Lemma remove_nops_preserves_wf :
+  forall tles p, Some p = entities_to_init tles ->
+                 exists p', Some p' = entities_to_init (remove_nops_entities tles).
+Proof.
+  intros. induction tles; try solve [inversion H].
+  simpl in H. destruct a; simpl.
+  destruct (raw_id_beq (dc_name (df_prototype defn)) (Name "main")); eauto.
+  destruct (df_instrs defn); try solve [inversion H].
+  simpl. destruct (remove_nops_block_instrs (blk_instrs b)); eapply ex_intro; eauto.
+Qed.
+
+Theorem remove_nops_block_scope :
+  forall b p instrs,
+    Some b =
+    List.find (fun b : block => raw_id_beq (bn p) (blk_id b))
+         (map remove_nops_block instrs) ->
+    exists b', Some b' = List.find (fun b : block => raw_id_beq (bn p) (blk_id b)) instrs /\ b = remove_nops_block b'.
+Proof.
+  intros. induction instrs; try solve [simpl in H; inversion H].
+  simpl in *. destruct (raw_id_beq (bn p) (blk_id a)); try (eapply IHinstrs; eapply H).
+  exists a. inversion H; split; eauto.
+Qed.
+
+(* Removing nops doesn't affect commands that aren't removed *)
+Theorem remove_nops_cmd_from_block :
+  forall p b b' x,
+    remove_nops_block b = b' ->
+    Some x = cmd_from_block (ins p) (fn p) (bn p) (blk_term_id b') (blk_instrs b') ->
+    Some x = cmd_from_block (ins p) (fn p) (bn p) (blk_term_id b) (blk_instrs b).
+Proof.
+  intros. unfold remove_nops_block in *. subst; simpl in *.
+  destruct b; simpl in *.
+  induction blk_instrs. simpl in *; inversion H0.
+  simpl in *. destruct a; simpl in *.
+  destruct i0; simpl in *. apply IHblk_instrs in H0.
+  (* Need uniqueness here *)
+Admitted.
+
+(* Intuitively,  if something is removed it is a NOP *)
+Theorem remove_nops_missing :
+  forall p b b' x,
+    remove_nops_block b = b' ->
+    Some x = cmd_from_block (ins p) (fn p) (bn p) (blk_term_id b) (blk_instrs b) ->
+    None = cmd_from_block (ins p) (fn p) (bn p) (blk_term_id b') (blk_instrs b') ->
+    exists p', x = Step INSTR_Nop p'.
+Proof.
+  intros. destruct b; simpl in *. generalize dependent b'.
+  induction blk_instrs; try solve [simpl in H0; inversion H0].
+  intro. destruct a.
+  simpl in H0. destruct (instr_id_eq_dec (ins p) i).
+  - intros. eapply IHblk_instrs; eauto.
+    + destruct i0; admit.
+    + admit.
+  - intros.
+    eapply IHblk_instrs; eauto.
+    destruct i0; eauto. simpl. unfold remove_nops_block in H. simpl in H.
+    subst. destruct i0; eauto. simpl in H1.
+    destruct (instr_id_eq_dec (ins p) i); eauto. inversion H1.
+Admitted.
+
+(* We also need a property that says something like:
+   If we remove nops and encounter something missing, we eventually
+   reach the command that we stepped to in the block with the NOPs 
+   removed, and only encountered NOPs in between.
+
+   Or: if the nop-removed cfg and regular cfg step to different things
+    from some state, then the regular cfg will eventually step to the
+    same state as the nop-removed cfg did after one step.
+
+   We don't want to state this as a coinductive property because it
+    inherently needs to be finite.
+   I'm not sure exactly how to phrase this.
+ *)
+CoFixpoint step_until_id id CFG (s : state) : D state :=
+  let '(p, e, c) := s in
+  if instr_id_eq_dec id (ins p) then
+    stepD CFG s
+  else bind (stepD CFG s) (step_until_id id CFG).
+
+(* Intuitively this is true because of the above lemma: that we only 
+   encounter NOPs *)
+Theorem remove_nops_finite_missing :
+  forall p p' tles CFG CFG' st next e c,
+    Some p = entities_to_init tles ->
+    Some p' = entities_to_init (remove_nops_entities tles) ->
+    TLE_to_cfg tles = Some CFG ->
+    TLE_to_cfg (remove_nops_entities tles) = Some CFG' ->
+    stepD CFG' st = Ret (next, e, c) ->
+    d_equiv (stepD CFG' st) (step_until_id (ins next) CFG st).
+Proof.
+Abort.
+
+(* Then the general idea of the proof would be that we destruct
+   the (code cfg). The result would then be either None or Some.
+   In the some case we can remove the thing that is the same and 
+   then apply the coinductive hypothesis.
+   In the None case, we use the remove_nops_finite_missing lemma to
+   say that we eventually reach the same state as on the NOP-removed
+   case.
+
+   A similar argument should apply in the constant propagation case
+   except you need to thread some more state through (information about
+   which constants were propagated away).
+ *)
+  
+Theorem remove_nops_scope :
+  forall p p' p'' tles CFG CFG' cmd,
+    Some p' = entities_to_init tles ->
+    Some p'' = entities_to_init (remove_nops_entities tles) ->
+    TLE_to_cfg tles = Some CFG ->
+    TLE_to_cfg (remove_nops_entities tles) = Some CFG' ->
+    code CFG' p = Some cmd -> code CFG p = Some cmd.
+Proof.
+  intros. unfold code in *; destruct CFG; destruct CFG'; simpl in *.
+  unfold TLE_to_cfg in *. rewrite <- H in H1; rewrite <- H0 in H2.
+  simpl in *. inversion H1; clear H1; inversion H2; clear H2.
+  rewrite <- H9 in H3. clear H7 H8 H10 H11 H H0 H5 H4.
+  generalize dependent code0. generalize dependent code. induction tles.
+  - intros. unfold entities_to_code in H3; simpl in H3. inversion H3. 
+  - intros. simpl. simpl in H3. destruct a; simpl in H3.
+    destruct (raw_id_beq (dc_name (df_prototype defn)) (fn p)).
+    + remember (find (fun b => raw_id_beq (bn p) (blk_id b)) (map remove_nops_block (df_instrs defn))).
+      destruct o; simpl in H3; try (solve [inversion H3]).
+      assert (Heqo' := Heqo); eauto.
+      eapply remove_nops_block_scope in Heqo'.
+      destruct Heqo' as [b']. destruct H. rewrite <- H; simpl.
+      admit.
+      
+    + eapply IHtles; eauto.
+Abort.
+      
+Theorem remove_nops_equiv :
+  forall p p' p'' cont env tles CFG CFG',
+    Some p' = entities_to_init tles ->
+    Some p'' = entities_to_init (remove_nops_entities tles) ->
+    TLE_to_cfg tles = Some CFG ->
+    TLE_to_cfg (remove_nops_entities tles) = Some CFG' ->
+    code CFG' p <> None ->
+    d_equiv (bind (stepD CFG (p, env, cont)) (sem CFG))
+            (bind (stepD CFG' (p, env, cont)) (sem CFG')).
+Proof.
+  intros. pcofix CIH. pfold. unfold TLE_to_cfg in *.
+  rewrite <- H in H1. rewrite <- H0 in H2. simpl in *.
+  inversion H1; clear H1. inversion H2; clear H2.
+ 
+  unfold stepD.
+  
+Abort.
+
+Theorem remove_nops_equiv :
+  forall st tles CFG, TLE_to_cfg tles = Some CFG ->
+                      exists cfg', TLE_to_cfg (remove_nops_entities tles) = Some cfg' /\
+                                   d_equiv (sem CFG st) (sem cfg' st).
+Proof.
+  intros. unfold TLE_to_cfg in H. remember (entities_to_init tles).
+  destruct o; simpl in H; try solve [inversion H].
+  assert (Heqo' := Heqo); eauto.
+  eapply remove_nops_preserves_wf in Heqo'; destruct Heqo' as [p'].
+  unfold TLE_to_cfg. rewrite <- H0; simpl.
+  eapply ex_intro; split; eauto.
+  inversion H; simpl; eauto. clear H. clear H2.
+  (* We do need at least some properties of the state here *)
+  rewrite sem_unfold. rewrite sem_unfold.
+  pcofix CIH.
+Abort.
